SecureMessaging.lean
@@ -48,6 +48,10 @@ import SecureMessaging.SCKA.Defs
 import SecureMessaging.SCKA.MLKEMBraid.Authenticator
 import SecureMessaging.SCKA.MLKEMBraid.Basic
 import SecureMessaging.SCKA.MLKEMBraid.Construction
+import SecureMessaging.SCKA.SPQR.Chunked
+import SecureMessaging.SCKA.SPQR.Construction
+import SecureMessaging.SCKA.SPQR.Correspondence
+import SecureMessaging.SCKA.SPQR.Instances
 import SecureMessaging.SCKA.SPQR.Unchunked
 import SecureMessaging.SCKA.OppUniKEM.Construction
 import SecureMessaging.SCKA.OppUniKEM.Correctness
